running some examples through

examples/algorithms/QuickSort.List.fst
@@ -18,25 +18,25 @@ type total_order (a:Type) (f: (a -> a -> Tot bool)) =
     /\ (forall a1 a2. f a1 a2 \/ f a2 a1)                       (* totality      *)
 
 
-val count : 'a -> list 'a -> Tot nat
-let rec count (x:'a) (l:list 'a) = match l with
+val count : #a:Type{hasEq a} -> a -> list a -> Tot nat
+let rec count (#a:Type{hasEq a}) (x:a) (l:list a) = match l with
   | hd::tl -> (if hd=x then 1 else 0) + count x tl
   | [] -> 0
 
 
-val mem_count : x:'a -> l:list 'a ->
+val mem_count : #a:Type{hasEq a} -> x:a -> l:list a ->
       Lemma (requires True) (ensures (mem x l == (count x l > 0)))
       [SMTPat (mem x l)] (decreases l)
-let rec mem_count x l = match l with
+let rec mem_count #a x l = match l with
   | [] -> ()
   | _::tl -> mem_count x tl
 
 
-val append_count: l:list 'a -> m:list 'a -> x:'a
+val append_count: #a:Type{hasEq a} -> l:list a -> m:list a -> x:a
                -> Lemma (requires True)
                         (ensures (count x (append l m) = (count x l + count x m)))
                         [SMTPat (count x (append l m))]
-let rec append_count l m x = match l with
+let rec append_count #a l m x = match l with
   | [] -> ()
   | hd::tl -> append_count tl m x
 
@@ -53,7 +53,7 @@ let rec partition p = function
 (* this is used only to speed things up *)
 type trigger (#a:Type) (x:a) = True
 
-val partition_lemma: f:('a -> Tot bool) -> l:list 'a -> Lemma (requires True)
+val partition_lemma: #a:Type{hasEq a} -> f:(a -> Tot bool) -> l:list a -> Lemma (requires True)
       (ensures (forall hi lo. (hi, lo) = partition f l
                 ==>  (length l = length hi + length lo
                  /\ (forall x.{:pattern (trigger x)}
@@ -62,7 +62,7 @@ val partition_lemma: f:('a -> Tot bool) -> l:list 'a -> Lemma (requires True)
                            /\  (mem x lo ==> not (f x))
                            /\  (count x l = count x hi + count x lo)))))
       [SMTPat (partition f l)]
-let rec partition_lemma f l = match l with
+let rec partition_lemma #a f l = match l with
     | [] -> ()
     | hd::tl -> cut (trigger hd); partition_lemma f tl
 
@@ -81,11 +81,11 @@ let rec sorted_app_lemma #a f l1 l2 pivot = match l1 with
     | [] -> if is_Cons l2 then cut (trigger (Cons.hd l2)) else ()
     | hd::tl -> cut (trigger hd); sorted_app_lemma f tl l2 pivot
 
-val sort: f:('a -> 'a -> Tot bool){total_order 'a f}
-       -> l:list 'a
-       -> Tot (m:list 'a{sorted f m /\ (forall i.{:pattern trigger i} trigger i ==> (count i l = count i m))})
+val sort: #a:Type{hasEq a} -> f:(a -> a -> Tot bool){total_order a f}
+       -> l:list a
+       -> Tot (m:list a{sorted f m /\ (forall i.{:pattern trigger i} trigger i ==> (count i l = count i m))})
               (decreases (length l))
-let rec sort f = function
+let rec sort #a f = function
   | [] -> []
   | pivot::tl ->
     let hi, lo = partition (f pivot) tl in
